Cslib.lean
@@ -46,6 +46,15 @@ public import Cslib.Computability.Machines.MultiTapeTuring.MoveRoutine
 public import Cslib.Computability.Machines.MultiTapeTuring.MulRoutine
 public import Cslib.Computability.Machines.MultiTapeTuring.PopRoutine
 public import Cslib.Computability.Machines.MultiTapeTuring.PushRoutine
+public import Cslib.Computability.Machines.MultiTapeTuring.Routines.Boolean
+public import Cslib.Computability.Machines.MultiTapeTuring.Routines.CaseDispatch
+public import Cslib.Computability.Machines.MultiTapeTuring.Routines.Erase
+public import Cslib.Computability.Machines.MultiTapeTuring.Routines.ListIteration
+public import Cslib.Computability.Machines.MultiTapeTuring.Routines.ListOps
+public import Cslib.Computability.Machines.MultiTapeTuring.Routines.MultiTape
+public import Cslib.Computability.Machines.MultiTapeTuring.Routines.Navigation
+public import Cslib.Computability.Machines.MultiTapeTuring.Routines.Put
+public import Cslib.Computability.Machines.MultiTapeTuring.Routines.Skip
 public import Cslib.Computability.Machines.MultiTapeTuring.Satisfiability
 public import Cslib.Computability.Machines.MultiTapeTuring.SequentialCombinator
 public import Cslib.Computability.Machines.MultiTapeTuring.StructuralMachines
